transformations/Moore2Mealy/theorems/WFStable.v
@@ -84,3 +84,132 @@ Proof.
   rewrite C in IN_MOORE.
   exact IN_MOORE.
 Qed.
+
+Lemma transition_source_glue_r_exists_stable m :
+  Moore.WF_transition_source_exists m ->
+  Moore.WF_transition_source_glue_r_exists m ->
+  Mealy.WF_transition_source_glue_r_exists (Semantics.execute Moore2Mealy.Moore2Mealy m).
+Proof.
+  intro WF0.
+  unfold 
+    Moore.WF_transition_source_glue_r_exists, 
+    Mealy.WF_transition_source_glue_r_exists.
+  intros WF_MOORE t IN_MEALY.
+
+  destruct t.
+  apply Links.source_link_bw in IN_MEALY ; auto.
+  destruct IN_MEALY as (s0 & C & IN_MOORE).
+  unfold Glue.trg.
+  apply WF_MOORE in IN_MOORE.
+  unfold Glue.trg in IN_MOORE.
+  apply Elements.state_element_fw in IN_MOORE.
+  rewrite C in IN_MOORE.
+  exact IN_MOORE.
+Qed.
+
+Lemma WF_target_stable m:
+  MooreWF.WF_transition_target_uniqueness m ->
+  Moore.WF_transition_target_glue_r_exists m ->
+  Moore.WF_transition_target_glue_l_exists m ->
+  Moore.WF_transition_target_exists m ->
+  Mealy.WF_transition_target_exists (Semantics.execute Moore2Mealy.Moore2Mealy m).
+Proof.
+  intros WF0 WF1 WF2.
+  unfold 
+    Moore.WF_transition_target_exists,
+    Mealy.WF_transition_target_exists.
+  intro WF.
+  intros t IN_MEALY.
+  apply Elements.transition_element_bw in IN_MEALY.
+  destruct IN_MEALY as (t0 & IN_MOORE & C).
+  apply WF in IN_MOORE.
+  destruct IN_MOORE as (s0 & G).
+  apply Moore.getTransition_target_inv in G.
+  apply Links.target_link_fw in G ; auto.
+  destruct G as (t' & C' & IN_MEALY).
+  rewrite C' in C.
+  PropUtils.inj C.
+  exists (Moore2Mealy.convert_state s0).
+  apply MealyWF.getTransition_target_some ; auto with wf ; [].
+  apply transition_target_glue_r_exists_stable in WF1.
+  apply WF1 in IN_MEALY.
+  exact IN_MEALY.
+Qed.
+
+#[global]
+Hint Resolve transition_target_glue_r_exists_stable transition_source_glue_r_exists_stable WF_target_stable : wf.
+
+
+Lemma determinist_stable m :
+  Moore.WF_transition_target_exists m ->
+  Moore.WF_transition_source_glue_r_exists m ->
+  MooreWF.state_id_uniqueness m ->
+  Moore.WF_transition_source_exists m ->
+  MooreWF.WF_transition_source_uniqueness m ->
+  MooreWF.determinist m ->
+  MealyWF.determinist (Semantics.execute  Moore2Mealy.Moore2Mealy m).
+Proof.
+  intros WF_1 WF_3 WF_4 WF_5 WF_6 WF_2.
+  unfold MealyWF.determinist.
+  intros s t1 t2 H1 H2 H4.
+  apply MealySemantics.State_out_transitions_inv in H1.
+  apply MealySemantics.State_out_transitions_inv in H2.
+  destruct H1 as (IN1 & G1).
+  destruct H2 as (IN2 & G2).
+  
+  apply Elements.transition_element_bw in IN1. 
+  apply Elements.transition_element_bw in IN2.
+  destruct IN1 as (mt1 & ? & ?).
+  destruct IN2 as (mt2 & ? & ?).
+(*  specialize (WF_2 mt1 mt2 H H1).*)
+  unfold Moore2Mealy.convert_transition in H0.
+  PropUtils.destruct_match_H H0 ; [ PropUtils.inj H0 | discriminate H0 ] ; simpl in *.
+  unfold Moore2Mealy.convert_transition in H2.
+  PropUtils.destruct_match_H H2 ; [ PropUtils.inj H2 | discriminate H2 ] ; simpl in *.
+
+  apply Mealy.getTransition_source_inv in G1.
+  apply Mealy.getTransition_source_inv in G2.
+  
+  apply Links.source_link_bw in G1 ; auto ; [].
+  apply Links.source_link_bw in G2 ; auto ; [].
+  simpl in G1, G2.
+  destruct G1 as (s01 & C1 & IN1).
+
+  destruct G2 as (s02 & C2 & IN2).
+
+  PropUtils.duplicate IN1 IN_S01.
+  apply WF_3 in IN_S01. simpl in IN_S01.
+
+  PropUtils.duplicate IN2 IN_S02.
+  apply WF_3 in IN_S02. simpl in IN_S02.
+
+
+  assert (s01 = s02). 
+  { eapply Elements.convert_state_injective ; eauto. 
+    congruence.
+  }
+  subst s02.
+  clear IN_S02.
+
+  assert (mt1 = mt2).
+  {
+    unfold MooreWF.determinist in WF_2.
+(*    destruct mt1 ; destruct mt2.*)
+
+    eapply WF_2 ; eauto ; [ | ].
+
+    + apply MooreSemantics.in_State_outTransitions ; auto.
+      (* on aimerait avoir déjà GettersCommut *)
+      apply MooreWF.getTransition_source_some ; eauto.
+      destruct mt1 ; exact IN1.
+    + apply MooreSemantics.in_State_outTransitions ; auto.
+      apply MooreWF.getTransition_source_some ; eauto.
+      destruct mt2 ; exact IN2.
+  }
+
+  subst mt2.
+  congruence.
+Qed.
+
+#[global]
+Hint Resolve determinist_stable : wf.
